equality on types etc

src/frontend/Ast.fst
@@ -18,8 +18,7 @@ let dummy_pos = {
   col=0;
 }
 
-noeq
-type withrange 'a = {
+noeq type withrange 'a = {
   v:'a;
   range:range
 }
@@ -44,6 +43,7 @@ type op =
   | GE
   | SizeOf
 
+noeq
 type expr' =
   | Constant of constant
   | Identifier of ident
@@ -52,12 +52,14 @@ type expr' =
 
 and expr = withrange expr'
 
+noeq
 type typ' =
   | Type_app : ident -> list expr -> typ'
 and typ = withrange typ'
 
 type param = typ & ident
 
+noeq
 type struct_field = {
   field_dependence:bool;
   field_ident:ident;
@@ -65,6 +67,7 @@ type struct_field = {
   field_constraint:option expr;
 }
 
+noeq
 type field' =
  | Field of struct_field
  | FieldComment of string
@@ -72,12 +75,14 @@ and field = withrange field'
 type case = expr & field
 type switch_case = expr & list case
 
+noeq
 type typedef_names = {
   typedef_name: ident;
   typedef_abbrev: ident;
   typedef_ptr_abbrev: ident
 }
 
+noeq
 type decl' =
   | Comment of string
   | Define: ident -> constant -> decl'
@@ -85,6 +90,28 @@ type decl' =
   | Record: typedef_names -> list param -> list field -> decl'
   | CaseType: typedef_names -> list param -> switch_case -> decl'
 and decl = withrange decl'
+
+let rec eq_expr (e1 e2:expr) : Tot bool (decreases e1) =
+  match e1.v, e2.v with
+  | Constant i, Constant j -> i = j
+  | Identifier i, Identifier j -> i.v = j.v
+  | This, This -> true
+  | App op1 es1, App op2 es2 ->
+    op1 = op2
+    && eq_exprs es1 es2
+  | _ -> false
+
+and eq_exprs (es1 es2:list expr) : Tot bool =
+  match es1, es2 with
+  | [], [] -> true
+  | hd1::es1, hd2::es2 -> eq_expr hd1 hd2 && eq_exprs es1 es2
+  | _ -> false
+
+let eq_typ (t1 t2:typ) : Tot bool =
+  let Type_app hd1 es1, Type_app hd2 es2 = t1.v, t2.v in
+  hd1.v = hd2.v
+  && eq_exprs es1 es2
+
 
 let rec print_expr (e:expr) : Tot string =
   match e.v with
@@ -101,3 +128,12 @@ let rec print_expr (e:expr) : Tot string =
   | App Or [e1; e2] ->
     Printf.sprintf "(%s || %s)" (print_expr e1) (print_expr e2)
   | _ -> "??"
+
+let print_typ t : ML string =
+  let Type_app i es = t.v in
+  match es with
+  | [] -> i.v
+  | _ ->
+    Printf.sprintf "%s(%s)"
+      i.v
+      (String.concat ", " (List.map print_expr es))
